Clean up DivDef

Nonlinear_Arithmetic/Div-Def.dfy
@@ -4,102 +4,50 @@
 //- Note this is consistent: -3 * -1 + 2 == 5
 
 module DivDef {
-/*
-function mod(x:int, m:int) : int
-  requires m > 0
-  decreases if x < 0 then (m - x) else x
-{
-  if x < 0 then
-    mod(m + x, m)
-  else if x < m then
-    x
-  else
-    mod(x - m, m)
+
+  function method div(x: int, d: int): int
+    requires d != 0
+  {
+    x / d
+  }
+
+  function method mod(x: int, d: int): int
+    requires d != 0
+  {
+    x % d
+  }
+
+  function method div_recursive(x: int, d: int): int
+    requires d != 0
+  {
+    if d > 0 then
+      div_pos(x, d)
+    else
+      -1 * div_pos(x, -1*d)
+  }
+
+  function method mod_recursive(x: int, d: int): int
+    requires d > 0
+    decreases if x < 0 then (d - x) else x
+  {
+    if x < 0 then
+      mod_recursive(d + x, d)
+    else if x < d then
+      x
+    else
+      mod_recursive(x - d, d)
+  }
+
+  function method div_pos(x:int, d:int) : int
+    requires d >  0
+    decreases if x < 0 then (d - x) else x
+  {
+    if x < 0 then
+      -1 + div_pos(x+d, d)
+    else if x < d then
+      0
+    else
+      1 + div_pos(x-d, d)
+  }
+
 }
-*/
-
-function div(x:int, d:int) : int
-  requires d != 0
-{
-  x/d
-}
-
-function mod(x:int, d:int) : int
-  requires d != 0
-{
-  x%d
-}
-
-function div_recursive(x:int, d:int) : int
-  requires d != 0
-{ INTERNAL_div_recursive(x,d) }
-
-function mod_recursive(x:int, d:int) : int
-  requires d > 0
-{ INTERNAL_mod_recursive(x,d) }
-
-function mod_boogie(x:int, y:int) : int
-  requires y != 0
-{ x % y } //- INTERNAL_mod_boogie(x,y) }
-
-function div_boogie(x:int, y:int) : int
-  requires y != 0
-{ x / y } //-{ INTERNAL_div_boogie(x,y) }
-
-function my_div_recursive(x:int, d:int) : int
-  requires d != 0
-{
-  if d > 0 then
-    my_div_pos(x, d)
-  else
-    -1 * my_div_pos(x, -1*d)
-}
-
-function my_div_pos(x:int, d:int) : int
-  requires d >  0
-  decreases if x < 0 then (d - x) else x
-{
-  if x < 0 then
-    -1 + my_div_pos(x+d, d)
-  else if x < d then
-    0
-  else
-    1 + my_div_pos(x-d, d)
-}
-
-function my_mod_recursive(x:int, m:int) : int
-  requires m > 0
-  decreases if x < 0 then (m - x) else x
-{
-  if x < 0 then
-    my_mod_recursive(m + x, m)
-  else if x < m then
-    x
-  else
-    my_mod_recursive(x - m, m)
-}
-
-
-//- Kept for legacy reasons:
-//-static function INTERNAL_mod_boogie(x:int, m:int) : int   { x % y }
-function INTERNAL_mod_recursive(x:int, m:int) : int  
-  requires m > 0
-{ my_mod_recursive(x, m) }
-
-//-static function INTERNAL_div_boogie(x:int, m:int) : int   { x / m }
-function INTERNAL_div_recursive(x:int, d:int) : int 
-  requires d != 0
-{ my_div_recursive(x, d) }
-
-
-/*
-ghost method mod_test()
-{
-  assert -3 % 5 == 2;
-  assert 10 % -5 == 0;
-  assert 1 % -5 == 1;
-  assert -3 / 5 == -1;
-}
-*/
-
-} 
